---
date: 2023-09-01
tags:
  - posts
  - misc
eleventyNavigation:
  parent: Deep Atmosphere HOMME
  key: Final init
layout: layouts/post.njk
---

Define `$$ \pi(\eta) = A(\eta) \pi_0 + B(\eta) \pi_s$$`

Suppose we are given `$$T(z), p(z)$$`, with `$$ \pi_s = \int_0^\infty \frac{p}{R_d T} \intd{z}$$`.
This needs only be calculated once.

In SA HOMME, we have `$$ `

Then we can define `$$ \pi'_s = \int_0^\infty \hat{r}^2 \frac{p}{R_d T} \intd{z}$$`,
with `$$\pi'(\eta) = A(\eta) \pi_0 + B(\eta) \pi'_s$$`. 

Then solve 


